ContextStore/StoreFilterMapKey.v
@@ -1,0 +1,42 @@
+(** * Generic stores: partial key projection *)
+
+From ContextBase Require Import Prelude LogicVar.
+From ContextStore Require Import StoreCore StoreKeyAction.
+
+Section StoreFilterMapKey.
+
+Context {V : Type} `{ValueSig V}.
+
+Definition storeA_filter_map_key
+    {K K' : Type} `{Countable K} `{Countable K'}
+    (f : K -> option K') (s : StoreA K) : StoreA K' :=
+  map_fold (fun k v (acc : gmap K' V) =>
+    match f k with
+    | Some k' => <[k' := v]> acc
+    | None => acc
+    end) ∅ s.
+
+Lemma storeA_filter_map_key_empty
+    {K K' : Type} `{Countable K} `{Countable K'}
+    (f : K -> option K') :
+  storeA_filter_map_key f (∅ : StoreA K) = (∅ : StoreA K').
+Proof.
+  unfold storeA_filter_map_key. reflexivity.
+Qed.
+
+Definition AtomStore : Type := @StoreA V atom _ _.
+Definition LVarStore : Type := @StoreA V logic_var _ _.
+
+Definition atom_store_to_lvar_store (s : AtomStore) : LVarStore :=
+  storeA_map_key LVFree s.
+
+Definition lvar_to_atom (η : gmap nat atom) (v : logic_var) : option atom :=
+  logic_var_to_atom η v.
+
+Definition lvar_store_open (η : gmap nat atom) (s : LVarStore) : AtomStore :=
+  storeA_filter_map_key (lvar_to_atom η) s.
+
+Definition lvar_store_to_atom_store (s : LVarStore) : AtomStore :=
+  lvar_store_open ∅ s.
+
+End StoreFilterMapKey.
