ContextTypeLanguage/theories/LtyEnvBind.v
@@ -196,7 +196,7 @@ Proof.
       * discriminate.
     + symmetry. apply lty_env_closed_lookup_bound_none. exact Hclosed.
   - unfold lty_env_shift, lty_env_shift_from.
-    unfold storeA_rekey.
+    unfold storeA_rekey, storeA_map_key.
     change ((kmap (M2:=gmap logic_var) (logic_var_shift_from 0) Σ) !!
       LVFree x = (Σ : gmap logic_var ty) !! LVFree x).
     change (LVFree x) with (logic_var_shift_from 0 (LVFree x)) at 1.
